Modify examples

example/Demo.hs
@@ -16,20 +16,33 @@ doubleRoot t = root t + root t
 
 -- Traced value.
 tracedTree :: Tree Integer
-tracedTree = Node (trace "Root" 1) [Node (trace "Child" 2) []]
+tracedTree = Node (trace "Root" 1) [error "Error!" []]
 
 -- Example Property
 prop_double_root_traced :: Property
 prop_double_root_traced = doubleRoot tracedTree === trace "Root" 2
 
--- Recursive function with sharing.
-doubleElems :: [Integer] -> Integer
-doubleElems []       = 0
-doubleElems (x : xs) = x + x + doubleElems xs
 
-prop_double_Elems :: Property
-prop_double_Elems = doubleElems [trace "eval 1" 1, trace "eval 2" 2]
-  === trace "eval 1" (trace "eval 2" 6)
+
+
+
+
+
+
+
+
+
+
+
+
+
+
+
+
+
+
+
+
 {-
 
 -- Optional
