example/Demo2.hs
@@ -1,0 +1,13 @@
+module Demo2 where
+
+import           Debug.Trace
+import           Test.QuickCheck
+
+-- Recursive function with sharing.
+doubleElems :: [Integer] -> Integer
+doubleElems []       = 0
+doubleElems (x : xs) = x + x + doubleElems xs
+
+prop_double_Elems :: Property
+prop_double_Elems = doubleElems [trace "eval 1" 1, trace "eval 2" 2]
+  === trace "eval 1" (trace "eval 2" 6)
