example/Proofs/DemoProofs2.v
@@ -1,0 +1,52 @@
+From Base Require Import Free Handlers.
+From Base Require Import Prelude.
+From Base Require Import Test.QuickCheck.
+From Base Require Import Free.Instance.Maybe Instance.Trace.
+
+From Generated Require Import Demo2.
+
+Require Import Coq.Lists.List.
+Import List.ListNotations.
+Open Scope Z.
+
+
+(*
+doubleElems :: [Integer] -> Integer
+doubleElems [] = 0
+doubleElems (x:xs) = x + x + doubleElems xs
+
+prop_double_elems = doubleElems [trace "eval 1" 1, trace "eval 2" 2]
+=== trace "eval 1" (trace "eval 2" 6)
+
+*)
+
+(* Call-by-need evaluation. *)
+Theorem theorem_double_Elems_cbneed : quickCheckHandle (prop_double_Elems _ _ Cbneed _)
+ HandlerMaybeShareTrace.
+Proof. simpl; unfold Search.collectMessages; simpl.
+reflexivity. Qed.
+
+(* Call-by-name evaluation. *)
+Theorem theorem_double_Elems_cbn : ~quickCheckHandle (prop_double_Elems _ _ Cbn _)
+ HandlerMaybeShareTrace.
+Proof. simpl; unfold Search.collectMessages; simpl.
+discriminate. Qed.
+
+(* Call-by-value evaluation. *)
+Theorem theorem_double_Elems_cbv : quickCheckHandle (prop_double_Elems _ _ Cbv _)
+ HandlerMaybeShareTrace.
+Proof. simpl; unfold Search.collectMessages; simpl.
+reflexivity. Qed.
+
+(* Ignore tracing log, only consider results. *)
+Theorem theorem_double_Elems_cbneed_no_trace : quickCheckHandle (prop_double_Elems _ _ Cbneed
+ {| trace _ _ x := x |} ) HandlerShareTrace.
+Proof. simpl; unfold Search.collectMessages; simpl.
+reflexivity. Qed.
+
+(* Ignore tracing log, only consider results, use the minimal handler. *)
+Theorem theorem_double_Elems_cbneed_no_trace_min_handler 
+  : quickCheckHandle (prop_double_Elems _ _ Cbneed
+     {| trace _ _ x := x |} ) HandlerShare.
+Proof. simpl; unfold Search.collectMessages; simpl.
+reflexivity. Qed.
